marshalling the PackedStringArray

lib/DataStructures/PackedKV.i.dfy
@@ -1,6 +1,9 @@
 include "PackedStringArray.i.dfy"
+include "../Base/total_order.i.dfy"
 
 module PackedKV {
+  import Keyspace = Lexicographic_Byte_Order
+
   datatype Pkv = Pkv(
       keys: PackedStringArray.Psa,
       values: PackedStringArray.Psa)
@@ -13,6 +16,16 @@ module PackedKV {
   predicate ValidMessageByteString(s: seq<byte>)
   {
     |s| <= ValueWithDefault.MaxLen()
+  }
+
+  predicate ValidKeyByteStringSeq(s: seq<seq<byte>>)
+  {
+    forall i | 0 <= i < |s| :: ValidKeyByteString(s[i])
+  }
+
+  predicate ValidMessageByteStringSeq(s: seq<seq<byte>>)
+  {
+    forall i | 0 <= i < |s| :: ValidMessageByteString(s[i])
   }
 
   predicate WF(pkv: Pkv) {
